coqjit/dynamic_proof.v
@@ -10,6 +10,7 @@ Require Import customSmallstep.
 Require Import monad_impl.
 Require Import internal_simulations.
 Require Import sem_properties.
+Require Import middle_end_proof.
 
 (* The number of optimizations left *)
 Definition optim_index: Type := nat.
@@ -109,52 +110,64 @@ Ltac destruct_exec_index :=
 
 (* Relating semantic states of the original program and dynamic states *)
 Inductive match_states: program -> dynamic_index -> mixed_state -> dynamic_state -> Prop :=
-| dynamic_match: forall p nc' ji sync sync' ms ms'
-               (INTERNAL_SIM: backward_internal_simulation' p p None None nocode nc' AnchorOff AnchorOff (jorder ji) (jrel ji))
+| dynamic_match: forall initp currentp nc' ji sync sync' ms ms'
+                   (STK_NO: stk_no_anchor (state_stack ms'))
+                   (SYNC_NO: synchro_no_anchor sync')
+                   (PGM_NO: no_anchor currentp)
+               (INTERNAL_SIM: backward_internal_simulation' initp currentp None None nocode nc' AnchorOff AnchorOff (jorder ji) (jrel ji))
                (INTERNAL_MATCH: (jrel ji) (jindex ji) (sync, ms) (sync', ms')),
-    match_states p ji
+    match_states initp ji
                  (sync, ms)
-                 (Dynamic p None sync' (ms', nc') (joptim ji)).
+                 (Dynamic currentp None sync' (ms', nc') (joptim ji)).
 
 
 Theorem dynamic_optim_correct:
   forall p,
+    no_anchor p ->
     backward_simulation (mixed_sem p None nocode AnchorOff)
                         (dynamic_sem p None).
 Proof.
-  intros p.
+  intros p NOANC.
   eapply Backward_simulation with (bsim_match_states:=match_states p) (bsim_order:=dynamic_order).
   - eapply dynamic_order_wf.
   - intros s1 H. exists (Dynamic p None (S_Call (ir_call (prog_main p) nil)) init_n_state 0). constructor.
   - intros s1 s2 H H0. inv H. inv H0. exists (nb_opt, mkindex refl_type refl_match_states tt refl_order wf_refl).
-    exists (S_Call (ir_call (prog_main p) nil), init_mutables). split; constructor. auto.
-    apply backward_refl. unfold jrel, jindex. simpl. constructor.
+    exists (S_Call (ir_call (prog_main p) nil), init_mutables). split; constructor; auto.
+    + simpl. constructor.
+    + simpl. auto.
+    + apply backward_refl.
+    + unfold jrel, jindex. simpl. constructor.
   - intros i s1 s2 r MATCH SAFE FINAL. inv FINAL. inv MATCH.
     eapply (match_final_states INTERNAL_SIM) in INTERNAL_MATCH; eauto. constructor.
   - intros i s1 s2 MATCH SAFE. inv MATCH. (* progress *)
     apply (progress INTERNAL_SIM) in INTERNAL_MATCH as [[retval FINAL]|[t [s2' STEP]]] ; auto.
     + left. simpl. exists retval. inv FINAL. constructor.
     + right. simpl. simpl in STEP. exists t. destruct s2' as [sync'' ms''].
-      exists (Dynamic p None sync'' (ms'', nc') (joptim i)). apply exe_step. auto. (* simulation diagram *)
+      exists (Dynamic currentp None sync'' (ms'', nc') (joptim i)). apply exe_step. auto. (* simulation diagram *)
   - intros s2 t s2' DYN_STEP ji s1 MATCH SAFE. inv MATCH. simpl in DYN_STEP. inv DYN_STEP.
-    + eapply (simulation INTERNAL_SIM) in MIXED; eauto. (* execution step *)
+    + assert (NO: stk_no_anchor (state_stack ms2) /\ synchro_no_anchor sy2).
+      { destruct ms', ms2. apply step_preserve_no_anchor in MIXED; auto.  }
+      eapply (simulation INTERNAL_SIM) in MIXED; eauto. (* execution step *)
       destruct MIXED as [i' [[sy1 ms1]  [[PLUS | [STAR ORDER]] MATCH]]].
       * exists (jupdate ji i'). exists (sy1, ms1). split; auto. unfold jupdate. erewrite optim_update.
-        constructor; auto.
+        destruct NO. constructor; auto. 
       * exists (jupdate ji i'). exists (sy1, ms1). split; auto. right. split; auto.
         ** destruct ji. eapply exec_decreases. simpl. constructor. auto. 
-        ** erewrite optim_update. constructor; auto.
-    + apply optimizer_correct in OPT; auto.
+        ** erewrite optim_update. destruct NO. constructor; auto.
+    + assert (NO: no_anchor newp).
+      { eapply optimize_no_anchor; eauto. }
+      apply optimizer_correct in OPT; auto.
       apply backward_eq in OPT. destruct OPT as [optidx [optorder [optms OPT_SIM]]].
       specialize (match_states_refl OPT_SIM). unfold call_refl, p_reflexive. intros REFL.
-      specialize (REFL (S_Call loc, ms')). exploit REFL. constructor.
+      specialize (REFL (S_Call loc, ms')). exploit REFL. constructor. auto.
+      
       intros [i2 OPT_MATCH].
       (* composing the two backward simulations *)
       eapply compose_backward_simulation' in OPT_SIM as NEW_SIM; eauto.
       2: { apply single_mixed. } 
       (* Constructing the new index, with a new relation and new order *)
       set (neword:= lex_ord (Relation_Operators.clos_trans (index_type (jexec ji)) (jorder ji)) optorder).
-      set (newms := bb_ms p None nc' AnchorOff (jrel ji) optms).
+      set (newms := bb_ms currentp None nc' AnchorOff (jrel ji) optms).
       assert (NEWWF: well_founded neword) by apply (order_wf NEW_SIM).
       fold neword in NEW_SIM. fold newms in NEW_SIM.
       (* constructing the new match *)
@@ -163,18 +176,19 @@ Proof.
       * right. split. apply star_refl. destruct ji. unfold jindex. simpl. apply optim_decreases.
         unfold joptim in H5. simpl in H5. rewrite <- H5. simpl. lia.
       * replace nb_opt with (Nat.pred (joptim ji)) by lia. econstructor; auto.
-        unfold jrel, jindex, jexec, newms. simpl. eapply bb_match_at'; eauto.
+        unfold jrel, jindex, jexec, newms.  simpl. eapply bb_match_at'; eauto.
 Qed.
 
 Corollary dynamic_input_correct:
   forall p,
+    no_anchor p ->
     backward_simulation (input_sem p)
                         (dynamic_sem p None).
 Proof.
-  intros p. eapply customSmallstep.compose_backward_simulation.
+  intros p NO. eapply customSmallstep.compose_backward_simulation.
   - apply single_dynamic.
   - eapply input_mixed. 
-  - apply dynamic_optim_correct. 
+  - apply dynamic_optim_correct. auto.
 Qed.
 
     
