coqjit/middle_end.v
@@ -1,0 +1,44 @@
+(* Middle-end optimizer *)
+(* Inerting Speculation in CoreIR programs *)
+
+Require Import RTL.
+Require Import IR.
+Require Import monad.
+Require Import common.
+Require Import Coqlib.
+Require Import backend.
+Require Import primitives.
+Require Import anchor_insertion.
+Require Import assume_insertion.
+Require Import anchor_removal.
+Require Import profiler_types.
+Require Import Errors.
+Require Import monad.
+
+(* Inserting Anchors in all functions according to the profiler wish *)
+Fixpoint process_anc_list (p:program) (l:list (fun_id * list label)): program :=
+  match l with
+  | nil => p
+  | (fid, anc_lbl)::l' => process_anc_list (safe_insert_anchor p fid anc_lbl) l'
+  end.
+
+(* Processing each middle_end optimization sugeested by the profiler *)
+(* Using the safe optimizations: if one fails, it is just ignored by the optimizer *)
+Fixpoint process_optim_list (p:program) (l:list (fun_id * middle_wish)): program :=
+  match l with
+  | nil => p
+  | (fid, AS_INS guard anc_lbl)::l' => process_optim_list (safe_insert_assume p fid guard anc_lbl) l'
+  end.
+
+Definition middle_end (ps:profiler_state) (p:program): res program :=
+    do optims <- OK (middle_end_suggestion ps);
+    do fs_list <- OK (anchors_to_insert ps);
+    do pfs <- OK (process_anc_list p fs_list);
+    do newp <- OK (process_optim_list pfs optims);
+    OK (lowering newp).
+
+(* An error in optimization should not stop the execution *)
+Definition safe_middle_end (ps:profiler_state) (p:program): program :=
+  safe_res (middle_end ps) p.
+
+
