coqjit/profiler_types.v
@@ -1,0 +1,24 @@
+(* The profiler types and parameters *)
+
+Require Import IR.
+Require Import common.
+
+
+
+(* The state of the profiler *)
+Parameter profiler_state: Type.
+(* Suggest a function to use the backend on *)
+Parameter backend_suggestion: profiler_state -> fun_id.
+
+(* the locations where the profiler wants to insert anchors *)
+Parameter anchors_to_insert : profiler_state -> list (fun_id * (list label)).
+
+(* The different kinds of middle-end Optimizations passes the profiler wishes to make *)
+Inductive middle_wish : Type :=
+| AS_INS: expr -> label -> middle_wish.
+(* later, we could add constprop, delayed assume insertion and inlining from CoreJIT *)
+
+(* The middle-end optimizations suggestions for the middle-end *)
+Parameter middle_end_suggestion: profiler_state -> list (fun_id * middle_wish).
+
+
